invariantes/ex3.dfy
@@ -1,20 +1,18 @@
-ghost function Fatorial(n:nat):nat
+ghost function Fat(n: nat): nat
 {
-    if n == 0
-    then 1
-    else n * Fatorial(n-1)
+  if n == 0 then 1 else n * Fat(n-1)
 }
 
-method Fat(n:nat) returns (f:nat)
-ensures f == Fatorial(n)
+method Fatorial(n:nat)  returns (r:nat)
+  ensures r == Fat(n)
 {
-    var i := 1;
-    f := 1;
-    while i <= n
-      invariant f == Fatorial(i-1)
-      invariant 1 <= i <= n+1
-    {
-        f := f * i;
-        i := i + 1;
-    }
+  var i := 1;
+  r := 1;
+  while i <= n
+    invariant 1 <= i <= n+1
+    invariant r == Fat(i-1)
+  {
+    r := r* i;
+    i := i + 1;
+  }
 }
