hoare/ex0.dfy
@@ -2,9 +2,12 @@ method Triple(x: int) returns (r: int)
   requires true
   ensures r == 3*x
 {
-    assert x+2*x == 3*x;
+    assert x+2*x == 3*x; //obtido pelo cálculo da precondição mais fraca via Floyd-Hoare
     var y := 2*x;
     assert x+y == 3*x;
     r := x + y;
     assert r == 3*x;
 }
+
+// A condição de verificação para a correção é:
+// true ==> x+2*x == 3*x
