introducao/ex1.dfy
@@ -1,7 +1,7 @@
 method Triple(x: int) returns (r: int)
-  requires true
+  requires true //pode ser removido, é a condição padrão
   ensures r == 3*x
 {
-    var y := 2*x;
-    r := x + y; //return x + y;
+  var y := 2*x;
+  r := x + y; //return x + y;
 }
