introducao/ex2.dfy
@@ -1,9 +1,10 @@
 method Triple(x: int) returns (r: int)
   ensures r == 3*x
 {
-    var y := Double(x); //A verificação depende apenas do contrato e não da implementação concreta; diz-se que métodos são opacos
-    r := x + y;
+  var y := Double(x);
+  r := x + y;
 }
 
 method Double(x: int) returns (r: int)
   ensures r == 2*x
+//A verificação depende apenas do contrato e não da implementação concreta; diz-se que métodos são opacos
