invariantes/ex1.dfy
@@ -1,13 +1,13 @@
 method Mult(x:nat, y:nat) returns (a:nat)
   ensures a == x * y
 {
-    var m:nat := x;
-    var n:nat := y;
-    a := 0;
-    while m > 0
-      invariant a + m * n == x * y
-    {
-        a := a + n;
-        m := m - 1;
-    }
+  var m:nat := x;
+  var n:nat := y;
+  a := 0;
+  while m > 0
+    invariant a + m * n == x * y
+  {
+    a := a + n;
+    m := m - 1;
+  }
 }
