invariantes/ex2.dfy
@@ -1,18 +1,18 @@
 ghost function Fat(n: nat): nat
 {
-   if n == 0 then 1 else n * Fat(n-1)
+  if n == 0 then 1 else n * Fat(n-1)
 }
 
 method Fatorial(n:nat)  returns (r:nat)
   ensures r == Fat(n)
 {
-    r := 1;
-    var i := 0;
-    while i < n
-      invariant i <= n
-      invariant r == Fat(i)
-    {
-        i := i + 1;
-        r := r * i;
-    }
+  r := 1;
+  var i := 0;
+  while i < n
+    invariant i <= n
+    invariant r == Fat(i)
+  {
+    i := i + 1;
+    r := r * i;
+  }
 }
