terminacao/ex1.dfy
@@ -2,7 +2,7 @@ function Somar(m:nat, n:nat):nat
   decreases m
   ensures Somar(m,n) == m+n
 {
-    if (m == 0)
-    then n
-    else Somar(m-1,n) + 1
+  if (m == 0)
+  then n
+  else Somar(m-1,n) + 1
 }
